Add congruence proofs

src/Core_Erlang_Equivalences.v
@@ -18,17 +18,31 @@ forall env eff res eff' id1 id2,
 <->
   |env, id1, e2, eff| -s> |id2, res, eff'|.
 
-Definition strongly_equivalent e1 e2 id1 id2 id1' id2' :=
-forall env eff res eff',
+Definition strongly_equivalent e1 e2 P1 P2 :=
+(forall env eff res eff' id1 id2,
+  P1 id1 ->
   |env, id1, e1, eff| -e> |id2, res, eff'|
-<->
-  |env, id1', e2, eff| -e> |id2', res, eff'|.
+->
+  exists id1' id2', |env, id1', e2, eff| -e> |id2', res, eff'|)
+/\
+(forall env eff res eff' id1' id2',
+  P2 id1' ->
+  |env, id1', e2, eff| -e> |id2', res, eff'|
+->
+  exists id1 id2, |env, id1, e1, eff| -e> |id2, res, eff'|).
 
-Definition strongly_equivalent_single e1 e2 id1 id2 id1' id2' :=
-forall env eff res eff',
+Definition strongly_equivalent_single e1 e2 P1 P2 :=
+(forall env eff res eff' id1 id2,
+  P1 id1 ->
   |env, id1, e1, eff| -s> |id2, res, eff'|
-<->
-  |env, id1', e2, eff| -s> |id2', res, eff'|.
+->
+  exists id1' id2', |env, id1', e2, eff| -s> |id2', res, eff'|)
+/\
+(forall env eff res eff' id1' id2',
+  P2 id1' ->
+  |env, id1', e2, eff| -s> |id2', res, eff'|
+->
+  exists id1 id2, |env, id1, e1, eff| -s> |id2, res, eff'|).
 
 (* Definition weakly_equivalent e1 e2 id1 id2 id1' id2' eff eff2 eff' eff2' :=
 forall env res,
@@ -57,19 +71,20 @@ Proof.
 Qed. *)
 
 (* Example exp_to_fun (e : Expression) (x : Var) (id id' : nat):
-  strongly_equivalent e (ELet [x] (EFun [] e) (EApp (EVar x) [])) (S id) id' id id'.
+  strongly_equivalent e (ELet [x] (EFun [] e) (EApp (EVar x) [])) (fun x => x > 0) (fun x => True).
 Proof.
   unfold strongly_equivalent.
   split; intros.
-  * eapply eval_single, eval_let; auto.
+  * exists (pred id1), id2. eapply eval_single, eval_let; auto.
     - apply eval_single, eval_fun.
     - reflexivity.
     - eapply eval_single, eval_app with (vals := []) (eff := []) (ids := []); auto.
       + eapply eval_single, eval_var. simpl. rewrite get_value_here. reflexivity.
       + auto.
-      + intros. inversion H0.
+      + intros. inversion H1.
       + unfold get_env. simpl. auto.
-  * inversion H. inversion H3; subst.
+        destruct id1. inversion H. simpl. auto.
+  * exists (S id1'), id2'. clear H. rename H0 into H. inversion H. inversion H3; subst.
     - pose (EE1 := element_exist 0 vals H18). inversion EE1. inversion H0. subst.
       inversion H18. apply eq_sym, length_zero_iff_nil in H2. subst.
       inversion H13. subst. inversion H5. subst.
@@ -104,15 +119,15 @@ Proof.
   * auto.
 Qed.
 
-(* Theorem strongly_equivalent_refl e :
-  forall id id',
-  strongly_equivalent e e id id' id id'.
+(* Theorem strongly_equivalent_refl e P :
+  strongly_equivalent e e P P.
 Proof.
   intros. unfold strongly_equivalent. split; intros.
-  * auto.
-  * auto.
-Qed.
+  * eexists. eexists. exact H.
+  * eexists. eexists. exact H.
+Qed. *)
 
+(*
 Theorem weakly_equivalent_refl e :
   forall id id' eff eff',
   weakly_equivalent e e id id' id id' eff eff' eff eff'.
@@ -129,15 +144,14 @@ Proof.
   split; apply H.
 Qed.
 
-(* Theorem strongly_equivalent_sym e1 e2 :
-  forall id1 id1' id2 id2',
-  strongly_equivalent e1 e2 id1 id1' id2 id2' -> strongly_equivalent e2 e1 id2 id2' id1 id1'.
+(* Theorem strongly_equivalent_sym e1 e2 P1 P2 :
+  strongly_equivalent e1 e2 P1 P2 -> strongly_equivalent e2 e1 P2 P1.
 Proof.
   unfold strongly_equivalent; intros.
   split; apply H.
-Qed.
+Qed. *)
 
-Theorem weakly_equivalent_sym e1 e2 :
+(* Theorem weakly_equivalent_sym e1 e2 :
   forall id1 id1' id2 id2' eff1 eff1' eff2 eff2',
   weakly_equivalent e1 e2 id1 id1' id2 id2' eff1 eff1' eff2 eff2' 
 ->
@@ -158,18 +172,18 @@ Proof.
   * apply H0 in H1. apply H in H1. auto.
 Qed.
 
-(* Theorem strongly_equivalent_trans e1 e2 e3 :
-  forall id1 id1' id2 id2' id3 id3',
-  strongly_equivalent e1 e2 id1 id1' id2 id2' -> strongly_equivalent e2 e3 id2 id2' id3 id3'
+(* Theorem strongly_equivalent_trans e1 e2 e3 P1 P2 P3 :
+  strongly_equivalent e1 e2 P1 P2 -> strongly_equivalent e2 e3 P2 P3
 ->
-  strongly_equivalent e1 e3 id1 id1' id3 id3'.
+  strongly_equivalent e1 e3 P1 P3.
 Proof.
-  unfold strongly_equivalent; intros.
+  unfold strongly_equivalent; intros; destruct H, H0.
   split; intros.
-  * apply H in H1. apply H0 in H1. auto.
+  * apply H in H3. destruct H3, H3. apply H0 in H3. auto. 2: auto.
   * apply H0 in H1. apply H in H1. auto.
-Qed.
+Qed. *)
 
+(*
 Theorem weakly_equivalent_trans e1 e2 e3 :
     forall id1 id1' id2 id2' id3 id3' eff1 eff1' eff2 eff2' eff3 eff3',
   weakly_equivalent e1 e2 id1 id1' id2 id2' eff1 eff1' eff2 eff2' ->
@@ -213,7 +227,7 @@ End equivalence_relation.
 
 Section congruence.
 
-Theorem ECons_congruence hd tl : forall hd' tl',
+Theorem ECons_congr hd tl : forall hd' tl',
   completely_equivalent hd hd' -> completely_equivalent tl tl'
 ->
   completely_equivalent_single (ECons hd tl) (ECons hd' tl').
@@ -230,7 +244,379 @@ Proof.
     - eapply eval_cons_hd_ex. apply H0 in H6. exact H6. apply H. assumption.
 Qed.
 
-Lemma value_exception_eq_dec (res res' : ValueSequence + Exception) : {res = res'} + {res <> res'}.
+Theorem ETuple_congr (l : list Expression) : forall (l' : list Expression),
+  length l = length l' ->
+  (forall i, i < length l -> completely_equivalent (nth i l ErrorExp) (nth i l' ErrorExp))
+->
+  completely_equivalent_single (ETuple l) (ETuple l').
+Proof.
+  assert (A : forall (l l' : list Expression) env id eff id' res eff',
+    length l = length l' ->
+    (forall i, i < length l -> completely_equivalent (nth i l ErrorExp) (nth i l' ErrorExp))
+    ->
+    |env, id, ETuple l, eff| -s> |id', res, eff'|
+    ->
+    |env, id, ETuple l', eff| -s> |id', res, eff'|). {
+  intros. unfold completely_equivalent, completely_equivalent_single in *.
+  * inversion H1; subst; rewrite H in *.
+    - eapply eval_tuple.
+      + exact H3.
+      + exact H4.
+      + exact H5.
+      + intros. pose (H6 i H2). apply H0 in e. 2: auto. auto.
+      + auto.
+      + auto.
+    - eapply eval_tuple_ex.
+      + exact H3.
+      + reflexivity.
+      + exact H5.
+      + exact H6.
+      + intros. pose (H7 j H2). apply H0 in e. 2: lia. auto.
+      + apply H0 in H10. auto. lia.
+  }
+  split; intros.
+  * eapply A. exact H. auto. auto.
+  * eapply A. symmetry. exact H. intros. rewrite <- H in *.
+    apply completely_equivalent_sym. auto. auto.
+Qed.
+
+Theorem ECall_congr (f : string) (l : list Expression) : forall (l' : list Expression),
+  length l = length l' ->
+  (forall i, i < length l -> completely_equivalent (nth i l ErrorExp) (nth i l' ErrorExp))
+->
+  completely_equivalent_single (ECall f l) (ECall f l').
+Proof.
+  assert (A : forall f (l l' : list Expression) env id eff id' res eff',
+  length l = length l' ->
+  (forall i, i < length l -> completely_equivalent (nth i l ErrorExp) (nth i l' ErrorExp))
+  ->
+  |env, id, ECall f l, eff| -s> |id', res, eff'|
+  ->
+  |env, id, ECall f l', eff| -s> |id', res, eff'|). {
+  intros. unfold completely_equivalent, completely_equivalent_single in *.
+  * inversion H1; subst; rewrite H in *.
+    - eapply eval_call.
+      + exact H4.
+      + exact H5.
+      + exact H6.
+      + intros. pose (H7 i H2). apply H0 in e. 2: auto. auto.
+      + auto.
+      + auto.
+    - eapply eval_call_ex.
+      + exact H4.
+      + reflexivity.
+      + exact H6.
+      + exact H7.
+      + intros. pose (H10 j H2). apply H0 in e. 2: lia. auto.
+      + apply H0 in H15. auto. lia.
+  }
+  split; intros.
+  * eapply A. exact H. auto. auto.
+  * eapply A. symmetry. exact H. intros. rewrite <- H in *.
+    apply completely_equivalent_sym. auto. auto.
+Qed.
+
+Theorem EPrimOp_congr (f : string) (l : list Expression) : forall (l' : list Expression),
+  length l = length l' ->
+  (forall i, i < length l -> completely_equivalent (nth i l ErrorExp) (nth i l' ErrorExp))
+->
+  completely_equivalent_single (EPrimOp f l) (EPrimOp f l').
+Proof.
+  assert (A : forall f (l l' : list Expression) env id eff id' res eff',
+  length l = length l' ->
+  (forall i, i < length l -> completely_equivalent (nth i l ErrorExp) (nth i l' ErrorExp))
+  ->
+  |env, id, EPrimOp f l, eff| -s> |id', res, eff'|
+  ->
+  |env, id, EPrimOp f l', eff| -s> |id', res, eff'|). {
+  intros. unfold completely_equivalent, completely_equivalent_single in *.
+  * inversion H1; subst; rewrite H in *.
+    - eapply eval_primop.
+      + exact H4.
+      + exact H5.
+      + exact H6.
+      + intros. pose (H7 i H2). apply H0 in e. 2: auto. auto.
+      + auto.
+      + auto.
+    - eapply eval_primop_ex.
+      + exact H4.
+      + reflexivity.
+      + exact H6.
+      + exact H7.
+      + intros. pose (H10 j H2). apply H0 in e. 2: lia. auto.
+      + apply H0 in H15. auto. lia.
+  }
+  split; intros.
+  * eapply A. exact H. auto. auto.
+  * eapply A. symmetry. exact H. intros. rewrite <- H in *.
+    apply completely_equivalent_sym. auto. auto.
+Qed.
+
+Theorem EApp_congr (exp : Expression) (l : list Expression) : forall (exp' : Expression) (l' : list Expression),
+  length l = length l' ->
+  completely_equivalent exp exp' ->
+  (forall i, i < length l -> completely_equivalent (nth i l ErrorExp) (nth i l' ErrorExp))
+->
+  completely_equivalent_single (EApp exp l) (EApp exp' l').
+Proof.
+  assert (A : forall exp exp' (l l' : list Expression) env id eff id' res eff',
+    length l = length l' ->
+    completely_equivalent exp exp' ->
+    (forall i, i < length l -> completely_equivalent (nth i l ErrorExp) (nth i l' ErrorExp))
+    ->
+    |env, id, EApp exp l, eff| -s> |id', res, eff'|
+    ->
+    |env, id, EApp exp' l', eff| -s> |id', res, eff'|).
+  {
+    unfold completely_equivalent.
+    intros. remember (EApp exp0 l0) as appl.
+    induction H2; inversion Heqappl; subst.
+    * eapply eval_app; rewrite H in *.
+      - exact H2.
+      - apply H0. exact H3.
+      - auto.
+      - exact H5.
+      - exact H6.
+      - intros. pose (H7 i H9). apply H1. auto. auto.
+      - auto.
+    * eapply eval_app_closure_ex. apply H0. exact H2.
+    * eapply eval_app_param_ex; rewrite H in *.
+      - exact H2.
+      - reflexivity.
+      - exact H4.
+      - exact H5.
+      - apply H0. auto. exact H6.
+      - intros. pose (H7 j H3). apply H1. lia. auto.
+      - apply H1. lia. auto.
+    * eapply eval_app_badfun_ex; rewrite H in *.
+      - exact H2.
+      - exact H3.
+      - exact H4.
+      - apply H0. auto. exact H5.
+      - intros. pose (H6 j H8). apply H1. lia. auto.
+      - congruence.
+      - auto.
+      - auto.
+    * eapply eval_app_badarity_ex; rewrite H in *.
+      - exact H2.
+      - exact H3.
+      - exact H4.
+      - apply H0. auto. exact H5.
+      - intros. pose (H6 j H8). apply H1. lia. auto.
+      - congruence.
+      - auto.
+      - auto.
+  }
+  intros. split.
+  * apply A; auto.
+  * apply A; try lia.
+    apply completely_equivalent_sym. auto.
+    intros. apply completely_equivalent_sym. apply H1. lia.
+Qed.
+
+Lemma match_clause_ith l : forall vals i gg ee bb,
+  match_clause vals l i = Some (gg,ee,bb)
+->
+  gg = nth i (map snd (map fst l)) ErrorExp /\
+  ee = nth i (map snd l) ErrorExp /\
+  bb = match_valuelist_bind_patternlist vals (nth i (map fst (map fst l)) []).
+Proof.
+  induction l; intros.
+  * inversion H.
+  * destruct i.
+    - destruct a. destruct p. simpl. simpl in H.
+      destruct (match_valuelist_to_patternlist vals l0); inversion H. auto.
+    - simpl in H. destruct a, p.
+      simpl. pose (IHl _ _ _ _ _ H). exact a.
+Qed.
+
+Theorem ECase_congr (exp : Expression) (l : list (list Pattern * Expression * Expression)) : forall (exp' : Expression) (l' : list (list Pattern * Expression * Expression)),
+  length l = length l' ->
+  completely_equivalent exp exp' ->
+  (forall i, i < length l -> completely_equivalent (nth i (map snd l) ErrorExp)
+                                                   (nth i (map snd (map fst l')) ErrorExp))
+->
+  completely_equivalent_single (ECase exp l) (ECase exp' l').
+Proof.
+  intros. unfold completely_equivalent, completely_equivalent_single in *.
+  split; intros. inversion H2; subst.
+  * eapply eval_case; rewrite H in *.
+    - apply H0. exact H5.
+    - exact H6.
+    - pose (match_clause_ith _ _ _ _ _ _ H7). destruct a. destruct H4.
+Admitted.
+
+Theorem ELet_congr (e1 e2 : Expression) vl : forall (e1' e2' : Expression),
+  completely_equivalent e1 e1' ->
+  completely_equivalent e2 e2'
+->
+  completely_equivalent_single (ELet vl e1 e2) (ELet vl e1' e2').
+Proof.
+  intros. unfold completely_equivalent, completely_equivalent_single in *.
+  split; intros.
+  * inversion H1; subst.
+    - eapply eval_let. apply H. exact H7. auto. apply H0. exact H13.
+    - eapply eval_let_ex. apply H. auto.
+  * inversion H1; subst.
+    - eapply eval_let. apply H. exact H7. auto. apply H0. exact H13.
+    - eapply eval_let_ex. apply H. auto.
+Qed.
+
+Theorem ESeq_congr (e1 e2 : Expression) (l : list Expression) : forall (e1' e2' : Expression),
+  completely_equivalent e1 e1' ->
+  completely_equivalent e2 e2'
+->
+  completely_equivalent_single (ESeq e1 e2) (ESeq e1' e2').
+Proof.
+  intros. unfold completely_equivalent, completely_equivalent_single in *.
+  split; intros.
+  * inversion H1; subst.
+    - eapply eval_seq. apply H. exact H6. auto. apply H0. exact H11.
+    - eapply eval_seq_ex. apply H. auto.
+  * inversion H1; subst.
+    - eapply eval_seq. apply H. exact H6. auto. apply H0. exact H11.
+    - eapply eval_seq_ex. apply H. auto.
+Qed.
+
+Theorem ELetRec_congr (exp : Expression) l : forall (exp' : Expression),
+  completely_equivalent exp exp'
+->
+  completely_equivalent_single (ELetRec l exp) (ELetRec l exp').
+Proof.
+  intros. unfold completely_equivalent, completely_equivalent_single in *.
+  split; intros.
+  * inversion H0. subst. eapply eval_letrec. apply H. exact H9.
+  * inversion H0. subst. eapply eval_letrec. apply H. exact H9.
+Qed.
+
+Theorem EMap_congr (l : list (Expression * Expression)) : 
+  forall (l' : list (Expression * Expression)),
+  length l = length l' ->
+  (let exps := make_map_exps l in
+   let exps' := make_map_exps l' in
+  forall i, i < length exps -> completely_equivalent (nth i exps ErrorExp) (nth i exps' ErrorExp))
+->
+  completely_equivalent_single (EMap l) (EMap l').
+Proof.
+  assert (A :
+    forall (l l' : list (Expression * Expression)) env id eff eff' id' res,
+    length l = length l' ->
+    (let exps := make_map_exps l in
+      let exps' := make_map_exps l' in
+       forall i, i < length exps -> completely_equivalent (nth i exps ErrorExp) (nth i exps' ErrorExp)) ->
+    |env, id, EMap l, eff | -s> |id', res, eff'|
+    ->
+    |env, id, EMap l', eff | -s> |id', res, eff' |
+  ). {
+  intros. unfold completely_equivalent, completely_equivalent_single in *.
+  * inversion H1; subst; rewrite H in *.
+    - unfold exps, vals in *.
+      eapply eval_map.
+      + exact H3.
+      + exact H4.
+      + exact H5.
+      + exact H6.
+      + intros. rewrite length_make_map_exps in H2, H7. rewrite H in H7.
+        pose (H7 i H2). apply H0 in e. exact e.
+        rewrite length_make_map_exps. lia.
+      + exact H8.
+      + auto.
+      + auto.
+      + auto.
+    - unfold exps, vals in *.
+      eapply eval_map_ex.
+      + exact H3.
+      + exact H4.
+      + exact H5.
+      + reflexivity.
+      + exact H7.
+      + intros.
+        pose (H8 j H2). apply H0 in e. exact e.
+        rewrite length_make_map_exps. lia.
+      + apply H0 in H11. auto. rewrite length_make_map_exps. lia.
+  }
+  split; intros.
+  * eapply A. exact H. auto. auto.
+  * eapply A. symmetry. exact H.
+    simpl. simpl in H0. rewrite length_make_map_exps. rewrite length_make_map_exps in H0.
+    intros. apply completely_equivalent_sym. apply H0. lia. auto.
+Qed.
+
+Theorem ETry_congr (e1 e2 e3 : Expression) vl1 vl2 : forall (e1' e2' e3' : Expression),
+  completely_equivalent e1 e1' ->
+  completely_equivalent e2 e2' ->
+  completely_equivalent e3 e3'
+->
+  completely_equivalent_single (ETry e1 vl1 e2 vl2 e3) (ETry e1' vl1 e2' vl2 e3').
+Proof.
+  assert (A : forall e1 e1' e2 e2' e3 e3' env id eff id' res eff',
+    completely_equivalent e1 e1' ->
+    completely_equivalent e2 e2' ->
+    completely_equivalent e3 e3' ->
+    |env, id, ETry e1 vl1 e2 vl2 e3, eff | -s> |id', res, eff'|
+    ->
+    |env, id, ETry e1' vl1 e2' vl2 e3', eff| -s> |id', res, eff'|
+  ).
+  {
+    intros. inversion H2; subst.
+    * eapply eval_try. apply H. exact H14. auto. apply H0. exact H16.
+    * eapply eval_catch. apply H. exact H14. apply H1. exact H15.
+  }
+  split; intros.
+  * eapply A. exact H. exact H0. exact H1. auto.
+  * eapply A.
+    1-3: apply completely_equivalent_sym.
+    exact H. exact H0. exact H1. auto.
+Qed.
+
+Theorem EValues_congr (l : list SingleExpression) : forall (l' : list SingleExpression),
+  length l = length l' ->
+  (forall i, i < length l -> completely_equivalent_single (nth i l ErrorExp) (nth i l' ErrorExp))
+->
+  completely_equivalent (EValues l) (EValues l').
+Proof.
+  assert (A : forall (l l' : list SingleExpression) env id eff id' res eff',
+    length l = length l' ->
+    (forall i, i < length l -> completely_equivalent_single (nth i l ErrorExp) (nth i l' ErrorExp))
+    ->
+    |env, id, EValues l, eff| -e> |id', res, eff'|
+    ->
+    |env, id, EValues l', eff| -e> |id', res, eff'|). {
+  intros. unfold completely_equivalent, completely_equivalent_single in *.
+  * inversion H1; subst; rewrite H in *.
+    - eapply eval_values.
+      + exact H3.
+      + exact H4.
+      + exact H5.
+      + intros. pose (H6 i H2). apply H0 in e. 2: auto. auto.
+      + auto.
+      + auto.
+    - eapply eval_values_ex.
+      + exact H3.
+      + reflexivity.
+      + exact H5.
+      + exact H6.
+      + intros. pose (H7 j H2). apply H0 in e. 2: lia. auto.
+      + apply H0 in H10. auto. lia.
+  }
+  split; intros.
+  * eapply A. exact H. auto. auto.
+  * eapply A. symmetry. exact H. intros. rewrite <- H in *.
+    apply completely_equivalent_single_sym. auto. auto.
+Qed.
+
+Theorem ESingle_congr (e : SingleExpression)  : forall (e': SingleExpression),
+  completely_equivalent_single e e'
+->
+  completely_equivalent (ESingle e) (ESingle e').
+Proof.
+  unfold completely_equivalent_single.
+  split; intros.
+  * inversion H0. eapply eval_single. subst. apply H. auto.
+  * inversion H0. eapply eval_single. subst. apply H. auto.
+Qed.
+
+(* Lemma value_exception_eq_dec (res res' : ValueSequence + Exception) : {res = res'} + {res <> res'}.
 Proof.
   set Value_eq_dec.
   repeat decide equality.
@@ -241,9 +627,9 @@ Proof.
   set Value_eq_dec.
   set string_dec.
   repeat decide equality.
-Defined.
+Defined. *)
 
-Theorem ECons_congruence_strongly hd tl : forall hd' tl' id id' id'' id2 id2' id2'',
+(* Theorem ECons_congruence_strongly hd tl : forall hd' tl' id id' id'' id2 id2' id2'',
   strongly_equivalent tl tl' id id' id2 id2' -> 
   strongly_equivalent hd hd' id' id'' id2' id2''
 ->
@@ -260,6 +646,6 @@ Proof.
     - eapply eval_cons. apply H0 in H6. exact H6. apply H in H11. assumption.
     - eapply eval_cons_tl_ex. apply H0. assumption.
     - eapply eval_cons_hd_ex. apply H0 in H6. exact H6. apply H. assumption.
-Qed.
+Qed. *)
 
 End congruence.
